[Yul] Simplify dynamic semantics.
Put the function state outside of the computation state, since it does not get
updated in the same way as the global and local state: it is an environment that
only needs to be passed as an input to the ACL2 execution functions, without
needing to be returned as output. (The addition of the functions in a block to
the function state is realized via a separate ACL2 function, which is called to
augment the function state.)

Adapt correctness proof of the DeadCodeEliminator transformation. This proof is
now simpler; the only "drawback" is that it no longer exhibits some of the proof
approaches needed for more complex transformations, namely the transformation of
computation states (because now we only need to transform the function state,
and not the computation state any more), but that more general approach is
clear, and will be used in upcoming proofs of other transformations.

books/kestrel/yul/language/dynamic-semantics.lisp
@@ -84,6 +84,36 @@
 
 ;;;;;;;;;;;;;;;;;;;;;;;;;;;;;;;;;;;;;;;;;;;;;;;;;;;;;;;;;;;;;;;;;;;;;;;;;;;;;;;;
 
+(fty::defprod cstate
+  :short "Fixtype of computational states."
+  :long
+  (xdoc::topstring
+   (xdoc::p
+    "According to [Yul: Specification of Yul: Formal Specification],
+     this consists of a local state object and a global state object.
+     The latter is generic in generic Yul.
+     For now, for simplicity, we ignore the global state completely,
+     but we plan to add that at some point."))
+  ((local lstate))
+  :tag :cstate
+  :pred cstatep)
+
+;;;;;;;;;;;;;;;;;;;;;;;;;;;;;;;;;;;;;;;;
+
+(fty::defresult cstate-result
+  :short "Fixtype of errors and computation states."
+  :ok cstate
+  :pred cstate-resultp)
+
+;;;;;;;;;;;;;;;;;;;;
+
+(defruled not-resulterrp-when-cstatep
+  (implies (cstatep x)
+           (not (resulterrp x)))
+  :enable (resulterrp cstatep))
+
+;;;;;;;;;;;;;;;;;;;;;;;;;;;;;;;;;;;;;;;;;;;;;;;;;;;;;;;;;;;;;;;;;;;;;;;;;;;;;;;;
+
 (fty::defprod funinfo
   :short "Fixtype of function information."
   :long
@@ -131,38 +161,19 @@
   :val-type funinfo
   :pred fstatep)
 
-;;;;;;;;;;;;;;;;;;;;;;;;;;;;;;;;;;;;;;;;;;;;;;;;;;;;;;;;;;;;;;;;;;;;;;;;;;;;;;;;
-
-(fty::defprod cstate
-  :short "Fixtype of computational states."
-  :long
-  (xdoc::topstring
-   (xdoc::p
-    "According to [Yul: Specification of Yul: Formal Specification],
-     this consists of a local state object and a global state object.
-     The latter is generic in generic Yul.
-     For now, for simplicity, we ignore the global state completely,
-     but we plan to add that at some point.
-     We also include the function state,
-     whose motivation is discussed in @(tsee fstate)."))
-  ((local lstate)
-   (functions fstate))
-  :tag :cstate
-  :pred cstatep)
-
 ;;;;;;;;;;;;;;;;;;;;;;;;;;;;;;;;;;;;;;;;
 
-(fty::defresult cstate-result
-  :short "Fixtype of errors and computation states."
-  :ok cstate
-  :pred cstate-resultp)
+(fty::defresult fstate-result
+  :short "Fixtype of errors and function states."
+  :ok fstate
+  :pred fstate-resultp)
 
 ;;;;;;;;;;;;;;;;;;;;
 
-(defruled not-resulterrp-when-cstatep
-  (implies (cstatep x)
+(defruled not-resulterrp-when-fstatep
+  (implies (fstatep x)
            (not (resulterrp x)))
-  :enable (resulterrp cstatep))
+  :enable (resulterrp fstatep))
 
 ;;;;;;;;;;;;;;;;;;;;;;;;;;;;;;;;;;;;;;;;;;;;;;;;;;;;;;;;;;;;;;;;;;;;;;;;;;;;;;;;
 
@@ -319,15 +330,14 @@
 
 ;;;;;;;;;;;;;;;;;;;;;;;;;;;;;;;;;;;;;;;;;;;;;;;;;;;;;;;;;;;;;;;;;;;;;;;;;;;;;;;;
 
-(define get-fun ((fun identifierp) (cstate cstatep))
+(define get-fun ((fun identifierp) (fstate fstatep))
   :returns (info funinfo-resultp)
-  :short "Obtain information about a function from the computation state."
+  :short "Obtain information about a function from the function state."
   :long
   (xdoc::topstring
    (xdoc::p
     "It is an error if the function does not exist."))
-  (b* ((fstate (cstate->functions cstate))
-       (fun-info (omap::in (identifier-fix fun) fstate))
+  (b* ((fun-info (omap::in (identifier-fix fun) (fstate-fix fstate)))
        ((unless (consp fun-info))
         (err (list :function-not-found (identifier-fix fun)))))
     (cdr fun-info))
@@ -335,9 +345,9 @@
 
 ;;;;;;;;;;;;;;;;;;;;;;;;;;;;;;;;;;;;;;;;;;;;;;;;;;;;;;;;;;;;;;;;;;;;;;;;;;;;;;;;
 
-(define add-fun ((fun identifierp) (info funinfop) (cstate cstatep))
-  :returns (new-cstate cstate-resultp)
-  :short "Add a function to the computation state."
+(define add-fun ((fun identifierp) (info funinfop) (fstate fstatep))
+  :returns (new-fstate fstate-resultp)
+  :short "Add a function to the function state."
   :long
   (xdoc::topstring
    (xdoc::p
@@ -345,27 +355,27 @@
    (xdoc::p
     "This is the dynamic counterpart of
      @(tsee add-funtype) in the static semantics."))
-  (b* ((fstate (cstate->functions cstate))
-       (fun-info (omap::in (identifier-fix fun) fstate))
+  (b* ((fun-info (omap::in (identifier-fix fun) (fstate-fix fstate)))
        ((when (consp fun-info))
         (err (list :function-already-exists (identifier-fix fun))))
        (new-fstate
-        (omap::update (identifier-fix fun) (funinfo-fix info) fstate))
-       (new-cstate (change-cstate cstate :functions new-fstate)))
-    new-cstate)
+        (omap::update (identifier-fix fun)
+                      (funinfo-fix info)
+                      (fstate-fix fstate))))
+    new-fstate)
   :hooks (:fix))
 
 ;;;;;;;;;;;;;;;;;;;;;;;;;;;;;;;;;;;;;;;;;;;;;;;;;;;;;;;;;;;;;;;;;;;;;;;;;;;;;;;;
 
-(define add-funs-in-statement-list ((stmts statement-listp) (cstate cstatep))
-  :returns (new-cstate cstate-resultp)
-  :short "Add all the functions in a block to the computation state."
+(define add-funs-in-statement-list ((stmts statement-listp) (fstate fstatep))
+  :returns (new-fstate fstate-resultp)
+  :short "Add all the functions in a block to the function state."
   :long
   (xdoc::topstring
    (xdoc::p
     "Just before executing a block,
      all the function definitions in the block
-     are added to computation states.
+     are added to the function state.
      This is because,
      as explained in [Yul: Specification of Yul: Scoping Rules],
      all the functions defined in a block are accessible in the whole block,
@@ -373,15 +383,15 @@
    (xdoc::p
     "This is the dynamic counterpart of
      @(tsee add-funtypes-in-statement-list) in the static semantics."))
-  (b* (((when (endp stmts)) (cstate-fix cstate))
+  (b* (((when (endp stmts)) (fstate-fix fstate))
        (stmt (car stmts))
        ((unless (statement-case stmt :fundef))
-        (add-funs-in-statement-list (cdr stmts) cstate))
+        (add-funs-in-statement-list (cdr stmts) fstate))
        (fdef (statement-fundef->get stmt))
-       ((ok cstate) (add-fun (fundef->name fdef)
+       ((ok fstate) (add-fun (fundef->name fdef)
                              (funinfo-for-fundef fdef)
-                             cstate)))
-    (add-funs-in-statement-list (cdr stmts) cstate))
+                             fstate)))
+    (add-funs-in-statement-list (cdr stmts) fstate))
   :hooks (:fix))
 
 ;;;;;;;;;;;;;;;;;;;;;;;;;;;;;;;;;;;;;;;;;;;;;;;;;;;;;;;;;;;;;;;;;;;;;;;;;;;;;;;;
@@ -404,6 +414,7 @@
      note that we implicitly check that the number of input variables
      matches the number of input values.
      The output variables are initialized to 0."))
+  (declare (ignore cstate))
   (b* ((cstate (change-cstate cstate :local nil))
        ((ok cstate) (add-vars-values in-vars in-vals cstate))
        ((ok cstate) (add-vars-values out-vars
@@ -440,7 +451,7 @@
   :ok eoutcome
   :pred eoutcome-resultp)
 
-;;;;;;;;;;;;;;;;;;;;;;;;;;;;;;
+;;;;;;;;;;;;;;;;;;;;
 
 (defruled not-resulterrp-when-eoutcomep
   (implies (eoutcomep x)
@@ -574,7 +585,10 @@
      which involves executing the statements in function bodies,
      which involves executing the expressions in the statements."))
 
-  (define exec-expression ((expr expressionp) (cstate cstatep) (limit natp))
+  (define exec-expression ((expr expressionp)
+                           (cstate cstatep)
+                           (fstate fstatep)
+                           (limit natp))
     :returns (outcome eoutcome-resultp)
     :short "Execute an expression."
     (b* (((when (zp limit)) (err (list :limit (expression-fix expr)))))
@@ -582,11 +596,12 @@
        expr
        :path (exec-path expr.get cstate)
        :literal (exec-literal expr.get cstate)
-       :funcall (exec-funcall expr.get cstate (1- limit))))
+       :funcall (exec-funcall expr.get cstate fstate (1- limit))))
     :measure (nfix limit))
 
   (define exec-expression-list ((exprs expression-listp)
                                 (cstate cstatep)
+                                (fstate fstatep)
                                 (limit natp))
     :returns (outcome eoutcome-resultp)
     :short "Execute a list of expressions."
@@ -603,16 +618,19 @@
          ((when (endp exprs)) (make-eoutcome :cstate (cstate-fix cstate)
                                              :values nil))
          ((ok (eoutcome outcome))
-          (exec-expression (car exprs) cstate (1- limit)))
+          (exec-expression (car exprs) cstate fstate (1- limit)))
          ((unless (equal (len outcome.values) 1))
           (err (list :not-single-value outcome.values)))
          (val (car outcome.values))
          ((ok (eoutcome outcome))
-          (exec-expression-list (cdr exprs) outcome.cstate (1- limit))))
+          (exec-expression-list (cdr exprs) outcome.cstate fstate (1- limit))))
       (make-eoutcome :cstate outcome.cstate :values (cons val outcome.values)))
     :measure (nfix limit))
 
-  (define exec-funcall ((call funcallp) (cstate cstatep) (limit natp))
+  (define exec-funcall ((call funcallp)
+                        (cstate cstatep)
+                        (fstate fstatep)
+                        (limit natp))
     :returns (outcome eoutcome-resultp)
     :short "Execute a function call."
     :long
@@ -626,13 +644,14 @@
     (b* (((when (zp limit)) (err (list :limit (funcall-fix call))))
          ((funcall call) call)
          ((ok (eoutcome outcome))
-          (exec-expression-list (rev call.args) cstate (1- limit))))
-      (exec-function call.name outcome.values outcome.cstate (1- limit)))
+          (exec-expression-list (rev call.args) cstate fstate (1- limit))))
+      (exec-function call.name outcome.values outcome.cstate fstate (1- limit)))
     :measure (nfix limit))
 
   (define exec-function ((fun identifierp)
                          (args value-listp)
                          (cstate cstatep)
+                         (fstate fstatep)
                          (limit natp))
     :returns (outcome eoutcome-resultp)
     :short "Execution a function on some values."
@@ -658,23 +677,24 @@
                                    (identifier-fix fun)
                                    (value-list-fix args))))
          (lstate-before (cstate->local cstate))
-         (fstate-before (cstate->functions cstate))
-         ((ok (funinfo info)) (get-fun fun cstate))
+         ((ok (funinfo info)) (get-fun fun fstate))
          ((ok cstate) (init-local info.inputs args info.outputs cstate))
          ((ok (soutcome outcome))
-          (exec-block info.body cstate (1- limit)))
+          (exec-block info.body cstate fstate (1- limit)))
          ((when (mode-case outcome.mode :break))
           (err (list :break-from-function (identifier-fix fun))))
          ((when (mode-case outcome.mode :continue))
           (err (list :continue-from-function (identifier-fix fun))))
          ((ok vals) (read-vars-values info.outputs outcome.cstate))
          (cstate (change-cstate outcome.cstate
-                                :local lstate-before
-                                :functions fstate-before)))
+                                :local lstate-before)))
       (make-eoutcome :cstate cstate :values vals))
     :measure (nfix limit))
 
-  (define exec-statement ((stmt statementp) (cstate cstatep) (limit natp))
+  (define exec-statement ((stmt statementp)
+                          (cstate cstatep)
+                          (fstate fstatep)
+                          (limit natp))
     :returns (outcome soutcome-resultp)
     :short "Execute a statement."
     :long
@@ -761,13 +781,13 @@
     (b* (((when (zp limit)) (err (list :limit (statement-fix stmt)))))
       (statement-case
        stmt
-       :block (exec-block stmt.get cstate (1- limit))
+       :block (exec-block stmt.get cstate fstate (1- limit))
        :variable-single
        (expression-option-case
         stmt.init
         :some
         (b* (((ok (eoutcome outcome))
-              (exec-expression stmt.init.val cstate (1- limit)))
+              (exec-expression stmt.init.val cstate fstate (1- limit)))
              ((unless (equal (len outcome.values) 1))
               (err (list :not-single-value outcome.values)))
              ((ok cstate)
@@ -782,7 +802,7 @@
             stmt.init
             :some
             (b* (((ok (eoutcome outcome))
-                  (exec-funcall stmt.init.val cstate (1- limit)))
+                  (exec-funcall stmt.init.val cstate fstate (1- limit)))
                  ((ok cstate)
                   (add-vars-values stmt.names outcome.values outcome.cstate)))
               (make-soutcome :cstate cstate :mode (mode-regular)))
@@ -796,7 +816,7 @@
        :assign-single
        (b* (((ok var) (path-to-var stmt.target))
             ((ok (eoutcome outcome))
-             (exec-expression stmt.value cstate (1- limit)))
+             (exec-expression stmt.value cstate fstate (1- limit)))
             ((unless (equal (len outcome.values) 1))
              (err (list :not-single-value outcome.values)))
             ((ok cstate)
@@ -807,64 +827,61 @@
              (err (list :non-multiple-variables stmt.targets)))
             ((ok vars) (paths-to-vars stmt.targets))
             ((ok (eoutcome outcome))
-             (exec-funcall stmt.value cstate (1- limit)))
+             (exec-funcall stmt.value cstate fstate (1- limit)))
             ((ok cstate)
              (write-vars-values vars outcome.values outcome.cstate)))
          (make-soutcome :cstate cstate :mode (mode-regular)))
        :funcall
        (b* (((ok (eoutcome outcome))
-             (exec-funcall stmt.get cstate (1- limit)))
+             (exec-funcall stmt.get cstate fstate (1- limit)))
             ((when (consp outcome.values))
              (err (list :funcall-statement-returns outcome.values))))
          (make-soutcome :cstate outcome.cstate :mode (mode-regular)))
        :if
        (b* (((ok (eoutcome outcome))
-             (exec-expression stmt.test cstate (1- limit)))
+             (exec-expression stmt.test cstate fstate (1- limit)))
             ((unless (equal (len outcome.values) 1))
              (err (list :if-test-not-single-value outcome.values)))
             (val (car outcome.values)))
          (if (equal val (value 0))
              (make-soutcome :cstate outcome.cstate :mode (mode-regular))
-           (exec-block stmt.body outcome.cstate (1- limit))))
+           (exec-block stmt.body outcome.cstate fstate (1- limit))))
        :for
        (b* ((vars-before (omap::keys (cstate->local cstate)))
-            (fstate-before (cstate->functions cstate))
             (stmts (block->statements stmt.init))
-            ((ok cstate) (add-funs-in-statement-list stmts cstate))
+            ((ok fstate) (add-funs-in-statement-list stmts fstate))
             ((ok (soutcome outcome))
-             (exec-statement-list stmts cstate (1- limit)))
+             (exec-statement-list stmts cstate fstate (1- limit)))
             ((when (mode-case outcome.mode :break))
              (err (list :break-from-for-init (statement-fix stmt))))
             ((when (mode-case outcome.mode :continue))
              (err (list :continue-from-for-init (statement-fix stmt))))
             ((when (mode-case outcome.mode :leave))
-             (b* ((cstate (change-cstate outcome.cstate
-                                         :functions fstate-before))
-                  (cstate (restrict-vars vars-before cstate)))
+             (b* ((cstate (restrict-vars vars-before outcome.cstate)))
                (make-soutcome :cstate cstate :mode (mode-leave))))
             ((ok (soutcome outcome))
              (exec-for-iterations stmt.test
                                   stmt.update
                                   stmt.body
                                   outcome.cstate
+                                  fstate
                                   (1- limit)))
             ((when (mode-case outcome.mode :break))
              (err (list :break-from-for (statement-fix stmt))))
             ((when (mode-case outcome.mode :continue))
              (err (list :continue-from-for (statement-fix stmt))))
-            (cstate (change-cstate outcome.cstate
-                                   :functions fstate-before))
-            (cstate (restrict-vars vars-before cstate)))
+            (cstate (restrict-vars vars-before outcome.cstate)))
          (make-soutcome :cstate cstate :mode outcome.mode))
        :switch
        (b* (((ok (eoutcome outcome))
-             (exec-expression stmt.target cstate (1- limit)))
+             (exec-expression stmt.target cstate fstate (1- limit)))
             ((unless (equal (len outcome.values) 1))
              (err (list :not-single-value outcome.values))))
          (exec-switch-rest stmt.cases
                            stmt.default
                            (car outcome.values)
                            outcome.cstate
+                           fstate
                            (1- limit)))
        :leave (make-soutcome :cstate (cstate-fix cstate)
                              :mode (mode-leave))
@@ -878,6 +895,7 @@
 
   (define exec-statement-list ((stmts statement-listp)
                                (cstate cstatep)
+                               (fstate fstatep)
                                (limit natp))
     :returns (outcome soutcome-resultp)
     :short "Execute a list of statements."
@@ -893,12 +911,15 @@
          ((when (endp stmts)) (make-soutcome :cstate (cstate-fix cstate)
                                              :mode (mode-regular)))
          ((ok (soutcome outcome))
-          (exec-statement (car stmts) cstate (1- limit)))
+          (exec-statement (car stmts) cstate fstate (1- limit)))
          ((unless (mode-case outcome.mode :regular)) outcome))
-      (exec-statement-list (cdr stmts) outcome.cstate (1- limit)))
+      (exec-statement-list (cdr stmts) outcome.cstate fstate (1- limit)))
     :measure (nfix limit))
 
-  (define exec-block ((block blockp) (cstate cstatep) (limit natp))
+  (define exec-block ((block blockp)
+                      (cstate cstatep)
+                      (fstate fstatep)
+                      (limit natp))
     :returns (outcome soutcome-resultp)
     :short "Execute a block."
     :long
@@ -916,13 +937,11 @@
        and we remove all the variables added by the block."))
     (b* (((when (zp limit)) (err (list :limit (block-fix block))))
          (vars-before (omap::keys (cstate->local cstate)))
-         (fstate-before (cstate->functions cstate))
          (stmts (block->statements block))
-         ((ok cstate) (add-funs-in-statement-list stmts cstate))
+         ((ok fstate) (add-funs-in-statement-list stmts fstate))
          ((ok (soutcome outcome))
-          (exec-statement-list stmts cstate (1- limit)))
-         (cstate (change-cstate outcome.cstate :functions fstate-before))
-         (cstate (restrict-vars vars-before cstate)))
+          (exec-statement-list stmts cstate fstate (1- limit)))
+         (cstate (restrict-vars vars-before outcome.cstate)))
       (make-soutcome :cstate cstate :mode outcome.mode))
     :measure (nfix limit))
 
@@ -930,6 +949,7 @@
                                (update blockp)
                                (body blockp)
                                (cstate cstatep)
+                               (fstate fstatep)
                                (limit natp))
     :returns (outcome soutcome-resultp)
     :short "Execute the iterations of a loop statement."
@@ -963,32 +983,33 @@
                                    (block-fix update)
                                    (block-fix body))))
          ((ok (eoutcome outcome))
-          (exec-expression test cstate (1- limit)))
+          (exec-expression test cstate fstate (1- limit)))
          ((unless (equal (len outcome.values) 1))
           (err (list :for-test-not-single-value outcome.values)))
          ((when (equal (car outcome.values) (value 0)))
           (make-soutcome :cstate outcome.cstate :mode (mode-regular)))
          ((ok (soutcome outcome))
-          (exec-block body outcome.cstate (1- limit)))
+          (exec-block body outcome.cstate fstate (1- limit)))
          ((when (mode-case outcome.mode :break))
           (make-soutcome :cstate outcome.cstate :mode (mode-regular)))
          ((when (mode-case outcome.mode :leave))
           (make-soutcome :cstate outcome.cstate :mode outcome.mode))
          ((ok (soutcome outcome))
-          (exec-block update outcome.cstate (1- limit)))
+          (exec-block update outcome.cstate fstate (1- limit)))
          ((when (mode-case outcome.mode :break))
           (err (list :break-from-for-update (block-fix update))))
          ((when (mode-case outcome.mode :continue))
           (err (list :continue-from-for-update (block-fix update))))
          ((when (mode-case outcome.mode :leave))
           (make-soutcome :cstate outcome.cstate :mode outcome.mode)))
-      (exec-for-iterations test update body outcome.cstate (1- limit)))
+      (exec-for-iterations test update body outcome.cstate fstate (1- limit)))
     :measure (nfix limit))
 
   (define exec-switch-rest ((cases swcase-listp)
                             (default block-optionp)
                             (target valuep)
                             (cstate cstatep)
+                            (fstate fstatep)
                             (limit natp))
     :returns (outcome soutcome-resultp)
     :short "Execute the rest of a switch statement,
@@ -1005,15 +1026,16 @@
                                    (swcase-list-fix cases)
                                    (block-option-fix default))))
          ((when (endp cases))
-          (block-option-case default
-                             :some (exec-block default.val cstate (1- limit))
-                             :none (make-soutcome :cstate (cstate-fix cstate)
-                                                  :mode (mode-regular))))
+          (block-option-case
+           default
+           :some (exec-block default.val cstate fstate (1- limit))
+           :none (make-soutcome :cstate (cstate-fix cstate)
+                                :mode (mode-regular))))
          ((swcase case) (car cases))
          ((ok caseval) (eval-literal case.value))
          ((when (value-equiv target caseval))
-          (exec-block case.body cstate (1- limit))))
-      (exec-switch-rest (cdr cases) default target cstate (1- limit)))
+          (exec-block case.body cstate fstate (1- limit))))
+      (exec-switch-rest (cdr cases) default target cstate fstate (1- limit)))
     :measure (nfix limit))
 
   :flag-local nil
@@ -1025,10 +1047,10 @@
   (fty::deffixequiv-mutual exec)
 
   (defruled statement-kind-when-mode-regular
-    (implies (and (soutcomep (exec-statement stmt cstate limit))
-                  (mode-case (soutcome->mode (exec-statement stmt cstate limit))
-                             :regular))
-             (and (not (equal (statement-kind stmt) :leave))
-                  (not (equal (statement-kind stmt) :break))
-                  (not (equal (statement-kind stmt) :continue))))
+    (b* ((outcome (exec-statement stmt cstate fstate limit)))
+      (implies (and (soutcomep outcome)
+                    (mode-case (soutcome->mode outcome) :regular))
+               (and (not (equal (statement-kind stmt) :leave))
+                    (not (equal (statement-kind stmt) :break))
+                    (not (equal (statement-kind stmt) :continue)))))
     :enable exec-statement))
